<?xml version="1.0"?>
<rdf:RDF xmlns="urn:absolute:temporary.crmtex/"
     xml:base="urn:absolute:temporary.crmtex/"
     xmlns:rdf="http://www.w3.org/1999/02/22-rdf-syntax-ns#"
     xmlns:terms="http://purl.org/dc/terms/"
     xmlns:owl="http://www.w3.org/2002/07/owl#"
     xmlns:xml="http://www.w3.org/XML/1998/namespace"
     xmlns:xsd="http://www.w3.org/2001/XMLSchema#"
     xmlns:skos="http://www.w3.org/2004/02/skos/core#"
     xmlns:rdfs="http://www.w3.org/2000/01/rdf-schema#"
     xmlns:dc="http://purl.org/dc/elements/1.1/">
    <owl:Ontology rdf:about="http://www.cidoc-crm.org/crmtex/">
        <owl:versionIRI rdf:resource="http://www.cidoc-crm.org/crmtex/0.1/"/>
        <owl:imports rdf:resource="http://erlangen-crm.org/current/"/>
        <dc:description rdf:datatype="http://www.w3.org/2000/01/rdf-schema#Literal">An Extension of CIDOC CRM to Model Ancient Textual Entities</dc:description>
        <terms:creator rdf:datatype="http://www.w3.org/2000/01/rdf-schema#Literal">Achille Felicetti</terms:creator>
        <dc:title rdf:datatype="http://www.w3.org/2000/01/rdf-schema#Literal">CRMtex</dc:title>
        <terms:creator rdf:datatype="http://www.w3.org/2000/01/rdf-schema#Literal">Francesca Murano</terms:creator>
    </owl:Ontology>



    <!--
    ///////////////////////////////////////////////////////////////////////////////////////
    //
    // Object Properties
    //
    ///////////////////////////////////////////////////////////////////////////////////////
     -->




    <!-- http://www.cidoc-crm.org/crmtex/TXP1_used_writing_system -->

    <owl:ObjectProperty rdf:about="http://www.cidoc-crm.org/crmtex/TXP1_used_writing_system">
      <rdfs:subPropertyOf rdf:resource="http://erlangen-crm.org/current/P33_used_specific_technique"/>
        <rdfs:domain rdf:resource="http://www.cidoc-crm.org/crmtex/TX2_Writing"/>
        <rdfs:range rdf:resource="http://www.cidoc-crm.org/crmtex/TX3_Writing_System"/>
        <rdfs:comment>Scope note:
          This property is intended to identify the specific instance of TX3 Writing System
          employed during the writing event that led to the creation of a TX1 Written Text.</rdfs:comment>
        <rdfs:label>TXP1 used writing system (writing system used for)</rdfs:label>
        <skos:notation>TXP1</skos:notation>
    </owl:ObjectProperty>



    <!-- http://www.cidoc-crm.org/crmtex/TXP2_is_included_within -->

    <owl:ObjectProperty rdf:about="http://www.cidoc-crm.org/crmtex/TXP2_includes">
        <rdfs:subPropertyOf rdf:resource="http://erlangen-crm.org/current/P56_bears_feature"/>
        <rdfs:range rdf:resource="http://www.cidoc-crm.org/crmtex/TX1_Written_Text"/>
        <rdfs:domain rdf:resource="http://www.cidoc-crm.org/crmtex/TX4_Writing_Field"/>
        <rdfs:comment>Scope note:
          This property is intended to describe the relation existing between a TX1 Written Text
          and the TX4 Writing Field, specifically created to accommodate the text, within which
          it is inscribed. This relation becomes quite relevant in the very frequent case where more
          than a single text is found on different areas of a specific support.</rdfs:comment>
        <rdfs:label>TXP2 includes (is included within)</rdfs:label>
        <skos:notation>TXP2</skos:notation>
    </owl:ObjectProperty>



    <!-- http://www.cidoc-crm.org/crmtex/TXP3_is_rendered_by_(renders) -->

    <owl:ObjectProperty rdf:about="http://www.cidoc-crm.org/crmtex/TXP3_rendered">
        <rdfs:subPropertyOf rdf:resource="http://erlangen-crm.org/current/P20_had_specific_purpose"/>
        <rdfs:range rdf:resource="http://www.cidoc-crm.org/crmtex/TX5_Reading"/>
        <rdfs:domain rdf:resource="http://www.cidoc-crm.org/crmtex/TX6_Transcription"/>
        <rdfs:comment>Scope note:
          This property is intended to emphasize the close connection for scientific purposes
          between the TX5 Reading and TX6 Transcription activities, by outlining, in particular, the accurate observation required by scholars in order to perform a valid transcription of
a the text being investigated.</rdfs:comment>
        <rdfs:label>TXP3 rendered (is rendered by)</rdfs:label>
        <skos:notation>TXP3</skos:notation>
    </owl:ObjectProperty>



    <!-- http://www.cidoc-crm.org/crmtex/TXP4_composes_(is_composed_by) -->

    <owl:ObjectProperty rdf:about="http://www.cidoc-crm.org/crmtex/TXP4_has_segment">
        <rdfs:subPropertyOf rdf:resource="http://erlangen-crm.org/current/P46_is_composed_of"/>
        <rdfs:domain rdf:resource="http://www.cidoc-crm.org/crmtex/TX7_Written_Text_Fragment"/>
        <rdfs:range rdf:resource="http://www.cidoc-crm.org/crmtex/TX1_Written_Text"/>
        <rdfs:comment>Scope note:
          This property is intended to correlate a text and the different parts of which a scholar can
          identify, such as: letters, words, lines, columns, pages, or any other scan that can be made
          by scholars because considered to have a particular relevance for the investigation of the
          text itself.</rdfs:comment>
        <rdfs:label>TXP4 has segment (is segment of)</rdfs:label>
        <skos:notation>TXP4</skos:notation>
    </owl:ObjectProperty>

    <!-- http://www.cidoc-crm.org/crmtex/TXP5 wrote (was written by) -->

    <owl:ObjectProperty rdf:about="http://www.cidoc-crm.org/crmtex/TXP5_wrote">
        <rdfs:subPropertyOf rdf:resource="http://erlangen-crm.org/current/P108_has_produced"/>
        <rdfs:domain rdf:resource="http://www.cidoc-crm.org/crmtex/TX2_Writing"/>
        <rdfs:range rdf:resource="http://www.cidoc-crm.org/crmtex/TX1_Written_Text"/>
        <rdfs:comment>Scope note:
          This property is used to describe in detail the close relationship between a text and the
  writing event that led to its production.</rdfs:comment>
        <rdfs:label>TXP5 wrote (was written by)</rdfs:label>
        <skos:notation>TXP5</skos:notation>
    </owl:ObjectProperty>

    <!-- http://www.cidoc-crm.org/crmtex/TXP6 encodes (is encoding of-->

    <owl:ObjectProperty rdf:about="http://www.cidoc-crm.org/crmtex/TXP6_encodes">
        <rdfs:subPropertyOf rdf:resource="http://erlangen-crm.org/current/P2_has_type"/>
        <rdfs:domain rdf:resource="http://www.cidoc-crm.org/crmtex/TX3_Writing_System"/>
        <rdfs:range rdf:resource="http://www.cidoc-crm.org/E33_Linguistic_Object"/>
        <rdfs:comment>Scope note:
          This property is used to indicate the language encoded by the TX3 Writing System and
used for writing, reading or rendering (i.e. transcribing) a TX1 Written Text. The
specification of the language is fundamental for understanding the writing phenomena
and the rules of the writing system used for the production or transcription of a specific
text.</rdfs:comment>
        <rdfs:label>TXP6 encodes (is encoding of)</rdfs:label>
        <skos:notation>TXP6</skos:notation>
    </owl:ObjectProperty>

    <!-- http://www.cidoc-crm.org/crmtex/TXP7 has item (is item of)-->

    <owl:ObjectProperty rdf:about="http://www.cidoc-crm.org/crmtex/TXP7_has_item">
        <rdfs:subPropertyOf rdf:resource="http://erlangen-crm.org/current/P106_is_composed_of"/>
        <rdfs:domain rdf:resource="http://www.cidoc-crm.org/crmtex/TX3_Writing_System"/>
        <rdfs:range rdf:resource="http://www.cidoc-crm.org/E33_Linguistic_Object"/>
        <rdfs:comment>Scope note:
          This property is used to state the (conceptual) belonging of a TX8 Grapheme to a given
TX3 Writing System.</rdfs:comment>
        <rdfs:label>TXP7 has item (is item of)</rdfs:label>
        <skos:notation>TXP7</skos:notation>
    </owl:ObjectProperty>

    <!-- http://www.cidoc-crm.org/crmtex/TXP8 has component (is component of)-->

    <owl:ObjectProperty rdf:about="http://www.cidoc-crm.org/crmtex/TXP8_has_component">
        <rdfs:subPropertyOf rdf:resource="http://erlangen-crm.org/current/P46_is_composed_of"/>
        <rdfs:domain rdf:resource="http://www.cidoc-crm.org/crmtex/TX1_Written_Text"/>
        <rdfs:range rdf:resource="http://www.cidoc-crm.org/crmtex/TX9_Glyph"/>
        <rdfs:comment>Scope note:
          This property is used to state the (physical) belonging of a TX9 Gliph to a given TX1
Written Text.</rdfs:comment>
        <rdfs:label>TXP8 has component (is component of)</rdfs:label>
        <skos:notation>TXP8</skos:notation>
    </owl:ObjectProperty>

    <!-- http://www.cidoc-crm.org/crmtex/TXP9 is encoded using (was used to encode)-->

    <owl:ObjectProperty rdf:about="http://www.cidoc-crm.org/crmtex/TXP9_is_encoded_using">
        <rdfs:domain rdf:resource="http://www.cidoc-crm.org/crmtex/TX1_Written_Text"/>
        <rdfs:range rdf:resource="http://www.cidoc-crm.org/crmtex/TX3_Writing_System"/>
        <rdfs:comment>Scope note:
          This property has the purpose of directly associating a TX1 Written Text with the TX3
Writing System from which the signs used for its writing and therefore incorporated in
the text have been taken. It is a shortcut of the more fully articulated path from TX1
Written Text, through TXP5 wrote (was written by), TX2 Writing, TXP1 used writing
system (writing system used for) to TX3 Writing System.</rdfs:comment>
        <rdfs:label>TXP9 is encoded using (was used to encode)</rdfs:label>
        <skos:notation>TXP9</skos:notation>
    </owl:ObjectProperty>

    <!-- http://www.cidoc-crm.org/crmtex/TXP10 read (was read by)-->

    <owl:ObjectProperty rdf:about="http://www.cidoc-crm.org/crmtex/TXP10_read">
        <rdfs:subPropertyOf rdf:resource="http://erlangen-crm.org/current/O8_observed"/>
        <rdfs:domain rdf:resource="http://www.cidoc-crm.org/crmtex/TX5_Reading"/>
        <rdfs:range rdf:resource="http://www.cidoc-crm.org/crmtex/TX1_Written_Text"/>
        <rdfs:comment>Scope note:
          This property links an instance of TX1 Written Text with a TX5 Reading event
carried out to investigate its intrinsic characteristics and to perform its decoding.</rdfs:comment>
        <rdfs:label>TXP10 read (was read by)</rdfs:label>
        <skos:notation>TXP10</skos:notation>
    </owl:ObjectProperty>


        <!-- http://www.cidoc-crm.org/crmtex/TXP11 transcribed (was transcribed by)-->

        <owl:ObjectProperty rdf:about="http://www.cidoc-crm.org/crmtex/TXP11_transcribed">
            <rdfs:subPropertyOf rdf:resource="http://erlangen-crm.org/current/P16_used_specific_object"/>
            <rdfs:domain rdf:resource="http://www.cidoc-crm.org/crmtex/TX6_Transcription"/>
            <rdfs:range rdf:resource="http://www.cidoc-crm.org/crmtex/TX8_Grapheme"/>
            <rdfs:comment>Scope note:
              This property highlights the specific way in which an activity of TX6 Transcription
results in the rendering of the specific TX8 Grapheme(s) of which an instance of TX1
Written Text is composed.</rdfs:comment>
            <rdfs:label>TXP11 transcribed (was transcribed by)</rdfs:label>
            <skos:notation>TXP11</skos:notation>
        </owl:ObjectProperty>


            <!-- http://www.cidoc-crm.org/crmtex/TXP12 has style (is style of)-->

            <owl:ObjectProperty rdf:about="http://www.cidoc-crm.org/crmtex/TXP11_transcribed">
                <rdfs:subPropertyOf rdf:resource="http://erlangen-crm.org/current/P33_used_specific_technique"/>
                <rdfs:domain rdf:resource="http://www.cidoc-crm.org/crmtex/TX1_Written_Text"/>
                <rdfs:range rdf:resource="http://www.cidoc-crm.org/crmtex/TX10_Style"/>
                <rdfs:comment>Scope note:
                  This property assigns information to a certain script in order to accurately determine
the style used for the realization of the written text. The TPX12.1 has type property of
TXP12 has style allows the nature of the style to be specified reading from domain to
range, for example to record the ductus, orientation or the linear system of the text.</rdfs:comment>
                <rdfs:label>TXP12 has style (is style of)</rdfs:label>
                <skos:notation>TXP12</skos:notation>
            </owl:ObjectProperty>

    <!--
    ///////////////////////////////////////////////////////////////////////////////////////
    //
    // Classes
    //
    ///////////////////////////////////////////////////////////////////////////////////////
     -->




    <!-- http://erlangen-crm.org/current/E25_Man-Made_Feature -->

    <owl:Class rdf:about="http://erlangen-crm.org/current/E25_Man-Made_Feature"/>



    <!-- http://www.cidoc-crm.org/crmtex/S19_Encounter_Event -->

    <owl:Class rdf:about="http://www.cidoc-crm.org/crmtex/S19_Encounter_Event">
        <rdfs:subClassOf rdf:resource="http://www.cidoc-crm.org/crmtex/S4_Observation"/>
        <rdfs:label rdf:datatype="http://www.w3.org/2000/01/rdf-schema#Literal">S19 Encounter Event</rdfs:label>
    </owl:Class>



    <!-- http://www.cidoc-crm.org/crmtex/S21_Measurement -->

    <owl:Class rdf:about="http://www.cidoc-crm.org/crmtex/S21_Measurement">
        <rdfs:subClassOf rdf:resource="http://www.cidoc-crm.org/crmtex/S4_Observation"/>
        <rdfs:label rdf:datatype="http://www.w3.org/2000/01/rdf-schema#Literal">S21 Measurement</rdfs:label>
    </owl:Class>



    <!-- http://www.cidoc-crm.org/crmtex/S4_Observation -->

    <owl:Class rdf:about="http://www.cidoc-crm.org/crmtex/S4_Observation">
        <rdfs:subClassOf rdf:resource="http://erlangen-crm.org/current/E13_Attribute_Assignment"/>
        <rdfs:comment rdf:datatype="http://www.w3.org/2000/01/rdf-schema#Literal">Scope note:
This class comprises the activity of gaining scientific knowledge about particular states of physical reality gained by empirical evidence, experiments and by measurements.
We define observation in the sense of natural sciences, as a kind of human activity: at some place and within some time-span, certain physical things and their behavior and interactions are observed, either directly by human sensory impression, or enhanced with tools and measurement devices.
The output of the internal processes of measurement devices that do not require additional human interaction are in general regarded as part of the observation and not as additional inference. Manual recordings may serve as additional evidence. Measurements and witnessing of events are special cases of observations. Observations result in a belief about certain propositions. In this model, the degree of confidence in the observed properties is regarded to be “true” by default, but could be described differently by adding a property P3 has note to an instance of S4 Observation, or by reification of the property O16 observed value.
Primary data from measurement devices are regarded in this model to be results of observation and can be interpreted as propositions believed to be true within the (known) tolerances and degree of reliability of the device.
Observations represent the transition between reality and propositions in the form of instances of a formal ontology, and can be subject to data evaluation from this point on. For instance, detecting an archaeological site on satellite images is not regarded as an instance of S4 Observation, but as an instance of S6 Data Evaluation. Rather, only the production of the images is regarded as an instance of S4 Observation.</rdfs:comment>
        <rdfs:label rdf:datatype="http://www.w3.org/2000/01/rdf-schema#Literal">S4 Observation</rdfs:label>
        <skos:notation rdf:datatype="http://www.w3.org/2000/01/rdf-schema#Literal">S4</skos:notation>
    </owl:Class>



    <!-- http://www.cidoc-crm.org/crmtex/TX10_Style -->

    <owl:Class rdf:about="http://www.cidoc-crm.org/crmtex/TX10_Style">
        <rdfs:subClassOf rdf:resource="http://erlangen-crm.org/current/E29_Design_or_Procedure"/>
        <rdfs:comment>Scope note:
Subclass of E29 Design or Procedure that describes styles and variations of texts,
including local script styles (Carolingian minuscule) and individual scribal hands. It
includes: the general appearance of the script, in terms of general design, aspects
related to a bilinear system (i.e. upper and lowercases), measures (i.e. large, medium
or small), shape and number of strokes forming a character, its order and direction. A
style includes also information about ductus (the direction the text is written), ligatures
and nexi (i.e. the connection between characters obtained tracing them without
detaching the writing instrument from the support and using one or more strokes in
common), and the writing angle (i.e. the position the writing instrument is located with
respect to the support). The style corresponds to fonts and their variations in modern
printing process.</rdfs:comment>
    </owl:Class>



    <!-- http://www.cidoc-crm.org/crmtex/TX1_Written_Text -->

    <owl:Class rdf:about="http://www.cidoc-crm.org/crmtex/TX1_Written_Text">
        <rdfs:subClassOf rdf:resource="http://erlangen-crm.org/current/E25_Man-Made_Feature"/>
        <rdfs:comment rdf:datatype="http://www.w3.org/2000/01/rdf-schema#Literal">Scope Note:
This class comprises visible set of symbols (glyphs or graphs) intentionally traced (i.e.
“written”) on some kind of physical support by using specific techniques and having
semiotic significance and the purpose of conveying a message towards a given
addressee or group of addressees.</rdfs:comment>
        <rdfs:label rdf:datatype="http://www.w3.org/2000/01/rdf-schema#Literal">TX1 Written Text</rdfs:label>
        <skos:notation rdf:datatype="http://www.w3.org/2000/01/rdf-schema#Literal">TX1</skos:notation>
    </owl:Class>



    <!-- http://www.cidoc-crm.org/crmtex/TX2_Writing -->

    <owl:Class rdf:about="http://www.cidoc-crm.org/crmtex/TX2_Writing">
        <rdfs:subClassOf rdf:resource="http://erlangen-crm.org/current/E12_Production"/>
        <rdfs:comment rdf:datatype="http://www.w3.org/2000/01/rdf-schema#Literal">Scope Note:
Subclass of F28 Expression Creation indicating the activity of physically creating a
text, using various techniques (painting, sculpture, etc.) and by means of specific tools,
on a given carrier in a non-mechanical way</rdfs:comment>
        <rdfs:label rdf:datatype="http://www.w3.org/2000/01/rdf-schema#Literal">TX2 Writing</rdfs:label>
        <skos:notation rdf:datatype="http://www.w3.org/2000/01/rdf-schema#Literal">TX2</skos:notation>
    </owl:Class>



    <!-- http://www.cidoc-crm.org/crmtex/TX3_Writing_System -->

    <owl:Class rdf:about="http://www.cidoc-crm.org/crmtex/TX3_Writing_System">
        <rdfs:subClassOf rdf:resource="http://erlangen-crm.org/current/E29_Design_or_Procedure"/>
        <rdfs:comment rdf:datatype="http://www.w3.org/2000/01/rdf-schema#Literal">Scope Note:
Subclass of E29 Design or Procedure refers to a conventional system consisting of a
set of signs (graphemes, TX8) used to codify a natural language, by means of specific
rules in the combination and phonological value assignment of the chosen graphemes.
As each code, a writing systems requires shared understanding between writers and
readers allowing the transmission of the message. It is used to produce a TX1 Written
Text during a TX2 Writing event.</rdfs:comment>
        <rdfs:label rdf:datatype="http://www.w3.org/2000/01/rdf-schema#Literal">TX3 Writing System</rdfs:label>
        <skos:notation rdf:datatype="http://www.w3.org/2000/01/rdf-schema#Literal">TX3</skos:notation>
    </owl:Class>



    <!-- http://www.cidoc-crm.org/crmtex/TX4_Writing_Field -->

    <owl:Class rdf:about="http://www.cidoc-crm.org/crmtex/TX4_Writing_Field">
        <rdfs:subClassOf rdf:resource="http://erlangen-crm.org/current/E25_Man-Made_Feature"/>
        <rdfs:comment rdf:datatype="http://www.w3.org/2000/01/rdf-schema#Literal">Scope Note:
Subclass of E25 Man-Made Feature, it is the portion of the physical support arranged
and usually reserved and delimited for the purpose of accommodating a written text,
highlighting and isolating it from the other parts of the object to which it belongs,
enhancing and guaranteeing its readability. This entity is paramount specially in
epigraphy, in which a specific element called “epigraphic field” has been defined by
the discipline itself. Its importance is also evident in papyrology and codicology, where
a clear distinction between area(s) containing the written text and empty parts of the
support (margins, intercolumnia, etc.) is significant for the definition of styles and
periods of the document.</rdfs:comment>
        <rdfs:label rdf:datatype="http://www.w3.org/2000/01/rdf-schema#Literal">TX4 Writing Field</rdfs:label>
        <skos:notation rdf:datatype="http://www.w3.org/2000/01/rdf-schema#Literal">TX4</skos:notation>
    </owl:Class>



    <!-- http://www.cidoc-crm.org/crmtex/TX5_Reading -->

    <owl:Class rdf:about="http://www.cidoc-crm.org/crmtex/TX5_Reading">
        <rdfs:subClassOf rdf:resource="http://www.cidoc-crm.org/crmtex/S4_Observation"/>
        <rdfs:comment rdf:datatype="http://www.w3.org/2000/01/rdf-schema#Literal">Scope Note:
Subclass of the S4 Observation, referring to the semiotic procedure of decoding (and
therefore understanding) a written text. This procedure can be carried out for scientific
purposes, in order to analyse and study the text according to different disciplinary
perspectives. The reading activity is thus intended as a specific observation (S4) in
which the decoding of the signs is performed, i.e. the linguistic value is recognised,
and the message is understood. Cases in which decoding does not happen (e.g., the
observer is able to describe the signs but not to assign a specific linguist value to them),
the S4 class could be used as it is. For study purposes, the reading procedure requires
a scientific autoptic examination of the text as preparatory action for the study. An
autoptic examination consists of an accurate analysis of the surface and the signs and
prescribes the use of specific tools and procedures, for establishing as faithfully as
possible the exact value of each sign drawn on the physical feature.</rdfs:comment>
        <rdfs:label rdf:datatype="http://www.w3.org/2000/01/rdf-schema#Literal">TX5 Reading</rdfs:label>
        <skos:notation rdf:datatype="http://www.w3.org/2000/01/rdf-schema#Literal">TX5</skos:notation>
    </owl:Class>



    <!-- http://www.cidoc-crm.org/crmtex/TX6_Transcription -->

    <owl:Class rdf:about="http://www.cidoc-crm.org/crmtex/TX6_Transcription">
        <rdfs:subClassOf rdf:resource="http://erlangen-crm.org/current/E7_Activity"/>
        <rdfs:comment rdf:datatype="http://www.w3.org/2000/01/rdf-schema#Literal">Scope Note:
Subclass of E7 Activity, referring to the activity of re-writing the text conducted by an
editor. This operation could involve a writing system (TX3) different from that of the
original text, implying a transposition of the sounds of a language from a writing
system to another one (e.g., Latin letters to render a Mycenaean text). For scientific
purposes, this operation often consists in a ‘transliteration’, because it implies a 1:1
relation between the signs of the two writing systems. The P16 used specific object
(was used for) property can be used to specify the role of the original graphemes during
the commuting operations.</rdfs:comment>
        <rdfs:label rdf:datatype="http://www.w3.org/2000/01/rdf-schema#Literal">TX6 Transcription</rdfs:label>
        <skos:notation rdf:datatype="http://www.w3.org/2000/01/rdf-schema#Literal">TX6</skos:notation>
    </owl:Class>



    <!-- http://www.cidoc-crm.org/crmtex/TX7_Written_Text_Fragment -->

    <owl:Class rdf:about="http://www.cidoc-crm.org/crmtex/TX7_Written_Text_Fragment">
        <rdfs:subClassOf rdf:resource="http://www.cidoc-crm.org/crmtex/TX1_Written_Text"/>
        <rdfs:comment rdf:datatype="http://www.w3.org/2000/01/rdf-schema#Literal">Scope Note:
Subclass of TX1 Written Text intended to identify portions of text considered to be of
particular significance by scholars, as witnesses of a certain meaning or bearers of a
particular phenomenon relevant to the investigation, study and understanding of the
ancient text. Examples of such text portions are: columns, fragments, sections,
paragraphs, as well as single words or letters, or other components of the written text.
To each of these entities can be associated a single production event (TX2) or
destruction event (E6), as in the case of letters or words damaged or worn by
atmospheric agents or human interventions, as well as specific conditions (E3) for
documenting its status during the observation process (S4). The relationship between
a written text (TX1) and its components is documented through the TXP4 has segment
property.</rdfs:comment>
        <rdfs:label rdf:datatype="http://www.w3.org/2000/01/rdf-schema#Literal">TX7 Written Text Segment</rdfs:label>
        <skos:notation rdf:datatype="http://www.w3.org/2000/01/rdf-schema#Literal">TX7</skos:notation>
    </owl:Class>



    <!-- http://www.cidoc-crm.org/crmtex/TX8_Grapheme -->

    <owl:Class rdf:about="http://www.cidoc-crm.org/crmtex/TX8_Grapheme">
        <rdfs:subClassOf rdf:resource="http://erlangen-crm.org/current/E90_Symbolic_Object"/>
        <rdfs:comment>Scope Note:
Subclass of E90 Symbolic Object used to represent the abstract units with distinctive
values in a given writing system. A grapheme is a character or sequence of characters
that functions as a distinct unit within an orthography. It may be a single character, a
multigraph, or a diacritic, but in all cases graphemes are defined in relation to the
particular orthography. Most graphemes represent a single phoneme, but some
represent a sequence of phonemes. For instance, the character sequence ‹ch› is often
used to represent the phoneme /tʃ/ in English, while the single letter ‹x› usually
represents the phoneme sequence /ks/. In a highly phonemic writing system, there is a
close correspondence between graphemes and phonemes. English (written with Latin
script) is an example of a writing system that is not highly phonemic, and therefore the
mappings between graphemes and phonemes are more complex. Graphemes are often
written enclosed in angle brackets (‹›).</rdfs:comment>
    </owl:Class>



    <!-- http://www.cidoc-crm.org/crmtex/TX9_Glyph -->

    <owl:Class rdf:about="http://www.cidoc-crm.org/crmtex/TX9_Glyph">
        <rdfs:subClassOf rdf:resource="http://erlangen-crm.org/current/E25_Man-Made_Feature"/>
        <rdfs:comment>Scope Note:
Subclass of E25 Man-Made Feature intended to represent the concrete manifestation
of single signs traced by the writer while codifying a linguistic expression. Glyphs are
typically observed by the scholar during a reading activity (TX5) carried out to decode
and recognise the graphemes (TX8) they represent.</rdfs:comment>
    </owl:Class>
</rdf:RDF>



<!-- Generated by the OWL API (version 4.2.6.20160910-2108) https://github.com/owlcs/owlapi -->
